thy/Primitive_Matchers/Common_Primitive_toString.thy
@@ -2,66 +2,13 @@ theory Common_Primitive_toString
 imports 
         "../Common/Lib_toString"
         "../Bitmagic/Lib_Word_toString"
+        "../Bitmagic/IpAddr_toString"
         Common_Primitive_Matcher
 begin
 
 
 section\<open>Firewall toString Functions\<close>
 
-fun dotteddecimal_toString :: "nat \<times> nat \<times> nat \<times> nat \<Rightarrow> string" where
-  "dotteddecimal_toString (a,b,c,d) = string_of_nat a@''.''@string_of_nat b@''.''@string_of_nat c@''.''@string_of_nat d"
-
-definition ipv4addr_toString :: "ipv4addr \<Rightarrow> string" where
-  "ipv4addr_toString ip = dotteddecimal_toString (dotdecimal_of_ipv4addr ip)"
-
-definition ipv6addr_toString :: "ipv6addr \<Rightarrow> string" where
-  "ipv6addr_toString ip = (
-    let partslist = ipv6_preferred_to_compressed (int_to_ipv6preferred ip);
-        (*add empty lists to the beginning and end if omission occurs at start/end
-          to join over ':' properly *)
-        fix_start = (\<lambda>ps. case ps of None#_ \<Rightarrow> None#ps | _ \<Rightarrow> ps);
-        fix_end = (\<lambda>ps. case rev ps of None#_ \<Rightarrow> ps@[None] | _ \<Rightarrow> ps)
-    in list_separated_toString '':''
-      (\<lambda>pt. case pt of None \<Rightarrow> ''''
-                    |  Some w \<Rightarrow> hex_string_of_word0 w)
-      ((fix_end \<circ> fix_start) partslist)
-    )"
-
-lemma "ipv6addr_toString (ipv6preferred_to_int (IPv6AddrPreferred 0x2001 0xDB8 0x0 0x0 0x8 0x800 0x200C 0x417A))
-            = ''2001:db8::8:800:200c:417a''" by eval --\<open>a unicast address\<close>
-
-lemma "ipv6addr_toString (ipv6preferred_to_int (IPv6AddrPreferred 0xFF01 0x0 0x0 0x0 0x0 0x0 0x0 0x0101)) =
-            ''ff01::101''" by eval --\<open>a multicast address\<close>
-
-lemma "ipv6addr_toString (ipv6preferred_to_int (IPv6AddrPreferred 0 0 0 0 0x8 0x800 0x200C 0x417A)) =
-             ''::8:800:200c:417a''" by eval
-
-lemma "ipv6addr_toString (ipv6preferred_to_int (IPv6AddrPreferred 0x2001 0xDB8 0 0 0 0 0 0)) =
-             ''2001:db8::''" by eval 
-
-lemma "ipv6addr_toString (ipv6preferred_to_int (IPv6AddrPreferred 0xFF00 0 0 0 0 0 0 0)) =
-             ''ff00::''" by eval --\<open>Multicast\<close>
-
-lemma "ipv6addr_toString (ipv6preferred_to_int (IPv6AddrPreferred 0xFE80 0 0 0 0 0 0 0)) =
-             ''fe80::''" by eval --\<open>Link-Local unicast\<close>
-
-lemma "ipv6addr_toString (ipv6preferred_to_int (IPv6AddrPreferred 0 0 0 0 0 0 0 0)) =
-             ''::''" by eval --\<open>unspecified address\<close>
-
-lemma "ipv6addr_toString (ipv6preferred_to_int (IPv6AddrPreferred 0 0 0 0 0 0 0 1)) =
-             ''::1''" by eval --\<open>loopback address\<close>
-
-lemma "ipv6addr_toString (ipv6preferred_to_int (IPv6AddrPreferred 0x2001 0xdb8 0x0 0x1 0x1 0x1 0x1 0x1)) =
-            ''2001:db8:0:1:1:1:1:1''" by eval --\<open>Section 4.2.2 of RFC5952\<close>
-
-
-
-text\<open>Generic function. Whenever possible, use IPv4 or IPv6 pretty printing!\<close>
-definition ipaddr_generic_toString :: "'i::len word \<Rightarrow> string" where
-  "ipaddr_generic_toString ip \<equiv>
-    ''[IP address ('' @ string_of_nat (len_of TYPE('i)) @ '' bit): '' @ dec_string_of_word0 ip @ '']''"
-
-lemma "ipaddr_generic_toString (ipv4addr_of_dotdecimal (192,168,0,1)) = ''[IP address (32 bit): 3232235521]''" by eval
 
 definition ipv4_cidr_toString :: "(ipv4addr \<times> nat) \<Rightarrow> string" where
   "ipv4_cidr_toString ip_n = (case ip_n of (base, n) \<Rightarrow>  (ipv4addr_toString base @''/''@ string_of_nat n))"
